Updated executable semantics

hol/p4_exec_semScript.sml
@@ -36,42 +36,98 @@ val find_clause_e_red = find_clause e_red_rules
 
 (***************************)
 
+(* Example of mutually recursive definition: 
+TotalDefn.multiDefine `
+ (test_func1 (0:num) = 0) /\
+ (test_func1 (SUC n) = test_func2 n) /\
+ (test_func2 (0:num) = 0) /\
+ (test_func2 (SUC n) = test_func1 n)
+`;
+*)
+
 (* NOTE: e_red is a small-step semantics *)
+
+val func_map = ``FEMPTY |+ ("f_x", (stmt_empty, ["x_inout", d_inout]))``;
 
 (* First, some kind of executable semantics definition *)
 (* No state modification, for now *)
 (* TODO: Write explicit NONE-reducing clauses for operands of wrong types?
  *       This would reduce the number of clauses pattern completion needs to add *)
-Definition e_exec:
+val e_stmt_exec = TotalDefn.multiDefine`
+ (* e_v is the fully reduced form of expression *)
  (e_exec (e_v v) (stacks:stacks) (status:status) =
-  SOME (e_v v))
+  SOME ((e_v v), stacks, status))
   /\
- (e_exec (e_var x) (stacks_tup curr_stack_frame call_stack) (status:status) =
-  SOME (e_v (lookup_vexp curr_stack_frame (e_var x))))
+ (********************)
+ (* Variable look-up *)
+ (e_exec (e_var x) (stacks_tup curr_stack_frame call_stack) status_running =
+  SOME ((e_v (lookup_vexp curr_stack_frame (e_var x))), stacks_tup curr_stack_frame call_stack, status_running))
+  /\
+ (*************************)
+ (* Function call-related *)
+(* TODO: Fix func_map in this definition... *)
+ (e_exec (e_func_call f e_l) (stacks_tup curr_stack_frame call_stack) status_running =
+  case FLOOKUP (^func_map) f of
+  | SOME (stmt, x_d_l) =>
+   if check_args_red (MAP SND x_d_l) e_l then
+    SOME (e_func_exec stmt,
+	  stacks_tup ([EL 0 curr_stack_frame]++[all_arg_update_for_newscope (MAP FST x_d_l) (MAP SND x_d_l) e_l curr_stack_frame])
+		     ((TL curr_stack_frame, called_function_name_function_name f)::call_stack),
+	  status_running)
+   else NONE
+  | NONE => NONE)
+  /\
+ (e_exec (e_func_exec stmt_empty) stacks (status_return v) =
+  SOME (e_v v, stacks, status_running))
+  /\
+ (e_exec (e_func_exec stmt) stacks (status:status) =
+  case stmt_exec stmt stacks status of
+  | SOME (stmt', stacks', status') => SOME (e_func_exec stmt', stacks', status')
+  | NONE => NONE)
+  /\
+ (***************************************)
+ (* Argument reduction of function call *)
+ (e_exec (e_func_call f e_l) (stacks_tup curr_stack_frame call_stack) status_running =
+  case FLOOKUP (^func_map) f of
+  | SOME (stmt, x_d_l) =>
+  (* TODO: Introduce result of unred_arg_index via a let statement, in order to not compute twice? *)
+   (case e_exec (EL (unred_arg_index (MAP SND x_d_l) e_l) e_l) (stacks_tup curr_stack_frame call_stack) status of
+    | SOME (e', stacks', status') => SOME (e_func_call f (LUPDATE e' (unred_arg_index (MAP SND x_d_l) e_l) e_l), stacks', status')
+    | NONE => NONE)
+(*
+   if check_args_red (MAP SND x_d_l) e_l then
+    SOME (e_func_exec stmt,
+	  stacks_tup ([EL 0 curr_stack_frame]++[all_arg_update_for_newscope (MAP FST x_d_l) (MAP SND x_d_l) e_l curr_stack_frame])
+		     ((TL curr_stack_frame, called_function_name_function_name f)::call_stack),
+	  status_running)
+   else NONE
+*)
+  | NONE => NONE)
   /\
  (********************)
  (* Unary arithmetic *)
  (e_exec (e_unop unop_neg (e_v (v_bool b))) (stacks:stacks) (status:status) =
-  SOME (e_v (v_bool ~b)))
+  SOME ((e_v (v_bool ~b)), stacks, status))
   /\
  (e_exec (e_unop unop_compl (e_v (v_bit bitv))) stacks status =
-  SOME (e_v (v_bit (bitv_bl_unop bnot bitv))))
+  SOME ((e_v (v_bit (bitv_bl_unop bnot bitv))), stacks, status))
   /\
  (e_exec (e_unop unop_neg_signed (e_v (v_bit bitv))) stacks status =
-  SOME (e_v (v_bit (bitv_unop unop_neg_signed bitv))))
+  SOME ((e_v (v_bit (bitv_unop unop_neg_signed bitv))), stacks, status))
   /\
  (e_exec (e_unop unop_un_plus (e_v (v_bit bitv))) stacks status =
-  SOME (e_v (v_bit bitv)))
+  SOME ((e_v (v_bit bitv)), stacks, status))
   /\
  (*****************************************)
  (* Argument reduction of unary operation *)
  (e_exec (e_unop unop e) (stacks:stacks) (status:status) =
   case e_exec e stacks status of
-  | SOME e' => SOME (e_unop unop e')
+  | SOME (e', stacks', status') => SOME ((e_unop unop e'), stacks', status')
   | NONE => NONE)
   /\
  (*********************)
  (* Binary arithmetic *)
+(*
  (e_exec (e_binop (e_v (v_bit bitv1)) binop_mul (e_v (v_bit bitv2))) (stacks:stacks) (status:status) =
   case bitv_binop binop_mul bitv1 bitv2 of
   | SOME bitv3 => SOME (e_v (v_bit bitv3))
@@ -153,18 +209,63 @@ Definition e_exec:
   | SOME e3 => SOME (e_binop e3 binop e2)
   | NONE => NONE)
   /\
+*)
  (e_exec _ stacks status = NONE)
-End
+  /\
+ (**************)
+ (* Statements *)
+ (**************)
+ (* empty_stmt is the fully reduced form of statement *)
+ (stmt_exec stmt_empty stacks status = SOME (stmt_empty, stacks, status)) /\
+ (*************************)
+ (* Function call-related *)
+(* TODO: Fix func_map in this definition... *)
+ (stmt_exec (stmt_ret (e_v v)) (stacks_tup curr_stack_frame call_stack) status_running =
+  case call_stack of
+  | ((curr_stack_frame', called_function_name_function_name f)::call_stack') =>
+   (case FLOOKUP (^func_map) f of
+   | SOME (stmt, x_d_l) => SOME (stmt_empty,
+				(stacks_tup (update_return_frame (MAP FST x_d_l) (MAP SND x_d_l) ((HD curr_stack_frame)::curr_stack_frame') curr_stack_frame)
+					    call_stack'),
+				status_return v)
+   | NONE => NONE)
+  | [] => NONE)
+  /\
+ (**************)
+ (* Assignment *)
+ (stmt_exec ((stmt_ass (lval_varname x) (e_v v)):stmt) (stacks_tup curr_stack_frame call_stack) (status:status) =
+  SOME (stmt_empty, (stacks_tup  (assign curr_stack_frame v x) call_stack), status))
+  /\
+ (stmt_exec ((stmt_ass lval_null (e_v v)):stmt) stacks (status:status) =
+  SOME (stmt_empty, stacks, status))
+  /\
+ (stmt_exec ((stmt_ass lval e):stmt) stacks (status:status) =
+  case e_exec e stacks status of
+  | SOME (e', stacks', status') => SOME (stmt_ass lval e', stacks', status')
+  | NONE => NONE)
+  /\
+ (************)
+ (* Sequence *)
+ (stmt_exec ((stmt_seq stmt_empty stmt):stmt) stacks (status:status) =
+  SOME (stmt, stacks, status))
+  /\
+ (stmt_exec ((stmt_seq stmt1 stmt2):stmt) stacks (status:status) =
+  case stmt_exec stmt1 stacks status of
+  | SOME (stmt1', stacks', status') => SOME (stmt_seq stmt1' stmt2, stacks', status')
+  | NONE => NONE)
+  /\
+ (stmt_exec (_:stmt) (stacks:stacks) (status:status) = NONE)
+`;
 
 (* Then, some kind of theorem that states equivalence
  * between executable semantics and ott-exported reduction rules.
  * For sketch, only soundness and not completeness *)
 (* TODO: Completeness *)
 (* TODO: Only running, for now... *)
-Theorem e_exec_subset_red:
- !(e:e) (e':e) stacks.
-  e_exec e stacks status_running = SOME e' ==>
-  e_red e stacks status_running e' stacks status_running
+Theorem e_exec_sound_red:
+ !(e:e) (e':e) stacks stacks' status status'.
+  e_exec e stacks status = SOME (e', stacks', status) ==>
+  e_red e stacks status e' stacks' status'
 Proof
 (* OLD version:
  Cases_on `e` >> Cases_on `e'` >> (
@@ -181,6 +282,14 @@ Proof
 cheat
 QED
 
+Theorem stmt_exec_sound_red:
+ !(stmt:stmt) (stmt':stmt) stacks stacks' status status'.
+  stmt_exec stmt stacks status = SOME (stmt', stacks', status) ==>
+  stmt_red stmt (state_tup stacks status) stmt' (state_tup stacks' status')
+Proof
+cheat
+QED
+
 Definition is_red:
  (is_red (e_v v) = T) /\
  (is_red _ = F)
@@ -189,8 +298,9 @@ End
 (* TODO: Instead of matching, put logic allowing only certain types of e_v in
  *       helper functions? *)
 (* Then, define an executable semantics which performs execution until finished. *)
-(* Note that all concrete operations remain esentially the same *)
-Definition e_clos_exec:
+(* Note that all concrete operations remain essentially the same *)
+val [e_clos_exec, stmt_clos_exec] = TotalDefn.multiDefine `
+ (* e_v is the fully reduced form of expression *)
  (e_clos_exec (e_v v) (stacks:stacks) (status:status) =
   e_exec (e_v v) stacks status)
   /\
@@ -211,7 +321,7 @@ Definition e_clos_exec:
  (* Unary operand reduction *)
  (e_clos_exec (e_unop unop e) (stacks:stacks) (status:status) =
   case e_clos_exec e stacks status of
-  | SOME ev => e_exec (e_unop unop ev) stacks status
+  | SOME (ev, stacks', status') => e_exec (e_unop unop ev) stacks' status'
   | NONE => NONE)
   /\
  (****************************)
@@ -245,13 +355,13 @@ Definition e_clos_exec:
 (* One clause, with conditions: *)
  (e_clos_exec (e_binop e1 binop e2) (stacks:stacks) (status:status) =
   case e_clos_exec e1 stacks status of
-  | SOME ev1 =>
+  | SOME (ev1, stacks', status') =>
    if is_red ev1
    then
-    (case e_clos_exec e2 stacks status of
-     | SOME ev2 =>
+    (case e_clos_exec e2 stacks' status' of
+     | SOME (ev2, stacks'', status'') =>
       if is_red ev2
-      then e_exec (e_binop ev1 binop ev2) stacks status
+      then e_exec (e_binop ev1 binop ev2) stacks'' status''
       else NONE
      | NONE => NONE)
    else NONE
@@ -259,12 +369,50 @@ Definition e_clos_exec:
   /\
  (* TODO: Ideally, the default case here should be "e_exec e stacks status",
   *       with all the recursive clauses needed defined above. *)
- (e_clos_exec _ stacks status = NONE)
-End
+ (e_clos_exec _ stacks status = NONE) /\
+ (**************)
+ (* Statements *)
+ (**************)
+ (stmt_clos_exec stmt_empty (stacks:stacks) (status:status) =
+  SOME (stmt_empty, stacks, status)) /\
+ (**************)
+ (* Assignment *)
+ (stmt_clos_exec ((stmt_ass lval e):stmt) stacks (status:status) =
+  case e_clos_exec e stacks status of
+  | SOME (ev, stacks', status') => stmt_exec (stmt_ass lval ev) stacks' status'
+  | NONE => NONE)
+  /\
+ (************)
+ (* Sequence *)
+ (stmt_clos_exec (stmt_seq stmt1 stmt2) stacks status =
+  case stmt_clos_exec stmt1 stacks status of
+  | SOME (empty_stmt, stacks', status') => stmt_clos_exec stmt2 stacks' status'
+  | NONE => NONE)
+  /\
+ (stmt_clos_exec (_:stmt) (stacks:stacks) (status:status) = NONE)
+`;
 (* TEST
+val bl0 = ``(w2v (0w:word32), 32)``;
 val bl1 = ``(w2v (1w:word32), 32)``;
 val bl2 = ``(w2v (16384w:word32), 32)``;
 
+val stacks = ``stacks_tup ([FEMPTY |+ ("x", ((v_bit (^bl0)), NONE))]:scope list) ([]:call_stack)``
+val status = ``status_running``
+
+(* Nested unary operations *)
+val e_un = ``(e_unop unop_compl (e_unop unop_compl (e_v (v_bit (^bl1)))))``;
+EVAL ``e_clos_exec (^e_un) stacks status``
+
+(* Single statements *)
+EVAL ``stmt_clos_exec (stmt_ass lval_null (^e_un)) (^stacks) (^status)``
+
+(* TODO: Simplifying multiple updates to the same finite map? *)
+EVAL ``stmt_clos_exec (stmt_ass (lval_varname "x") (^e_un)) (^stacks) (^status)``
+
+(* Sequence of statements *)
+EVAL ``stmt_clos_exec (stmt_seq (stmt_ass (lval_varname "x") (^e_un)) (stmt_ass (lval_varname "x") (e_v (v_bit (^bl2))) )) (^stacks) (^status)``
+
+(* Nested binary operations *)
 EVAL ``e_clos_exec (e_binop (e_v (v_bit (^bl1))) binop_add (e_v (v_bit (^bl2)))) stacks status``
    
 *)
@@ -283,18 +431,39 @@ val (e_clos_sem_rules, e_clos_sem_ind, e_clos_sem_cases) = Hol_reln`
 ( ( e_clos_red e stacks status_running e'' stacks'' status_running )))
 `;
 
+val (stmt_clos_sem_rules, stmt_clos_sem_ind, stmt_clos_sem_cases) = Hol_reln`
+(* Base clause: *)
+(! (stmt:stmt) (state:state) (stmt':stmt) (state':state).
+( ( stmt_red stmt state stmt' state' )) ==> 
+( ( stmt_clos_red stmt state stmt' state' )))
+(* Inductive clause: *)
+/\ (! (stmt:stmt) (state:state) (stmt':stmt) (state':state) (stmt'':stmt) (state'':state).
+(( ( stmt_red stmt state stmt' state' )) /\ 
+( ( stmt_clos_red stmt' state' stmt'' state'' ))) ==> 
+( ( stmt_clos_red stmt state stmt'' state'' )))
+`;
+
 (* Then, prove that the multi-step executable semantics is sound with respect to the
  * closure of the small-step reduction *)
 
-Theorem e_exec_clos_sound_red:
- !(e:e) (e':e) stacks.
-  e_exec_clos e stacks status_running = SOME e' ==>
-  e_clos_red e stacks status_running e' stacks status_running
+Theorem e_clos_exec_sound_red:
+ !(e:e) (e':e) stacks status stacks' status'.
+  e_clos_exec e stacks status = SOME (e', stacks', status') ==>
+  e_clos_red e stacks status e' stacks' status'
+Proof
+ cheat
+QED
+
+Theorem stmt_clos_exec_sound_red:
+ !(stmt:stmt) (stmt':stmt) stacks status stacks' status'.
+  stmt_clos_exec stmt stacks status = SOME (stmt', stacks', status') ==>
+  stmt_clos_red stmt (state_tup stacks status) stmt' (state_tup stacks' status')
 Proof
  cheat
 QED
 
 (* Then, some kind of (multi-step) CakeML-adjusted executable semantics definition *)
+(* TODO:
 Definition e_exec_cake:
  (e_exec_cake (e_unop unop_neg (e_v (v_bool b))) (stacks:stacks) (status:status) =
    SOME (e_v (v_bool ~b)))
@@ -318,5 +487,6 @@ Theorem sem_expr_exe_cake_equiv:
 Proof
  cheat
 QED
+*)
 
 val _ = export_theory ();
